\documentclass[]{IEEEtran}
\usepackage{amsmath}
\usepackage{listings}

\lstset{
frame=single, 
breaklines=true,
columns=fullflexible
}

\begin{document}

\begin{center}
\huge Assignment 1\\
\\*
\\*

\large Shreeprasad Bhat\\
\normalize AI20MTECH14011\\
\end{center}
\\
\begin{abstract}
This document illustrates scalar and vector products of two vectors
\end{abstract}
\\
\\
\\
Download python code from :
\begin{lstlisting}
https://github.com/shreeprasadbhat/matrix-theory/tree/master/assignment1/codes
\end{lstlisting}
%
\\

\textbf{Problem}\\
\\
Find scalar and vector products of the two vectors\\
\\
$$a &= \begin{bmatrix}
    3\\
    -4\\
    5
    \end{bmatrix},
b &= \begin{bmatrix}
    -2\\
    1\\
    -3
    \end{bmatrix}$$
\\
\\

\textbf{Solution} :\\
\textbf{Scalar product} :\\
  $$a\;.\;b \; &= \; 
  \begin{bmatrix}
  a_1\\
  a_2\\
  a_3
  \end{bmatrix} \; .\; 
  \begin{bmatrix}
  b_1\\
  b_2\\
  b_3
  \end{bmatrix}
  \; &= \; (a_1 \times b_1\;+\;a_2 \times b_2\;+\;a_3 \times b_3)$$\\
  Substituting a_1=3, \;a_2=-4, \;a_3=5 \;and\; b_1=-2,\;b_2=1,\;b_3=-3\\
  \\
  $$ &= \;\begin{bmatrix}
    3\\
    -4\\
    5
    \end{bmatrix} \; . \;
    \begin{bmatrix}
    -2\\ 1\\ -3 
    \end{bmatrix}\\$$
    \\
    $$ &\; = \; (3 \times -2)\; + \;(-4 \times 1)\;+\;(5 \times -3)$$
    \\
    $$ &= -25$$\\\\  
\textbf{Vector product} :\\
The\;vector\; cross\; product\; also\; can\; be\; expressed\; as\; the\; product\; of\; a\; skew-symmetric\; matrix\; and\; a\; vector\\\\
$$a\; \times \; b \; = \;
\begin{bmatrix}
0 & -a_3 & a_2\\
a_3 & 0 & -a_1\\
-a_2 & a_1 & 0
\end{bmatrix}
\end{bmatrix}
\begin{bmatrix}
b_1\\
b_2\\
b_3
\end{bmatrix}
\end{bmatrix}\\
\\\\Substituting a_1=3, \;a_2=-4, \;a_3=5 \;and\; b_1=-2,\;b_2=1,\;b_3=-3\\
\\$$a \; \times \; b \; &=  \;
    \begin{bmatrix}
    0 & -5 & -4\\
    5 & 0 & -3\\
    4 & 3 & 0
    \end{bmatrix}
    \begin{bmatrix}
    -2\\
    1\\
    -3
    \end{bmatrix}\\$$
    \\
    \\$$&= 
    \begin{bmatrix}
    (0 \times -2) \; + \; (-5 \times 1) \; + \; (-4 \times -3)\\
    (5 \times -2) \; + \; (0 \times 1) \; + \; (-3 \times -3)\\
    (4 \times -2) \; + \; (3 \times 1) \; + (0 \times -3)
    \end{bmatrix}
    \;&=\;\begin{bmatrix}
    7\\
    -1\\
    -5
    \end{bmatrix}
    $$

    
\end{document}